theories/Labelled_Transition_System/Examples_of_LTS/ACCS/ACCS_Must_Characterization.v
@@ -39,5 +39,3 @@ Proof.
 Qed.
 
 End ACCS_Must_Alt_Corollary.
-
-
