theories/Labelled_Transition_System/Examples_of_LTS/VACCS/VACCS_Must_Characterization.v
@@ -23,31 +23,15 @@
 From stdpp Require Import gmap gmultiset.
 
 From TestingTheory Require Import VACCS_ta_tc_gen DefinitionAS Equivalence Must 
-  ForwarderConstruction ParallelLTSConstruction InteractionBetweenLts Bisimulation.
+  ForwarderConstruction ParallelLTSConstruction InteractionBetweenLts Bisimulation
+  Completeness InputOutputActions Lts_OBA_FB MultisetLTSConstruction Lts_Finite_Output_Chain gLts.
 
 Module Type VACCS_Must_Alt_Corollary.
 Include VACCS_ta_tc.
 
 Corollary bhv_iff_ctx_VACCS (p q : proc) : p ⊑ₘᵤₛₜᵢ q <-> p ▷ ∅ ≼ₐₛ q ▷ ∅.
 Proof.
-  split.
-  - intro Hyp. eapply @equivalence_acc_set_and_must_i; eauto.
-
-    exact VACCS_gLtsFiniteImage. exact VACCS_gLtsFiniteImage. exact VACCS_gLtsFiniteImage.
-    exact Interaction_between_FW_VACCS_and_VACCS. exact Interaction_between_FW_VACCS_and_VACCS.
-    exact gen_conv_gen_spec_conv_inst.
-    exact gen_acc_gen_spec_acc_inst.
-    exact VACCS_gLtsOBAFB. exact VACCS_gFiniteOutputChain_LtsOba.
-
-
-  - intro Hyp. eapply @equivalence_acc_set_and_must_i in Hyp; eauto.
-
-    exact VACCS_gLtsFiniteImage. exact VACCS_gLtsFiniteImage. exact VACCS_gLtsFiniteImage.
-    exact Interaction_between_FW_VACCS_and_VACCS. exact Interaction_between_FW_VACCS_and_VACCS.
-    exact FinitaryAbsVACCS. exact FinitaryAbsVACCS.
-    exact gen_conv_gen_spec_conv_inst.
-    exact gen_acc_gen_spec_acc_inst.
-    exact VACCS_gLtsOBAFB. exact VACCS_gFiniteOutputChain_LtsOba.
+  eapply equivalence_acc_set_and_must_i.
 Qed.
 
 End VACCS_Must_Alt_Corollary.
