theories/Labelled_Transition_System/Examples_of_LTS/VCCS/VCCS_Instance.v
@@ -4448,7 +4448,7 @@ Next Obligation.
   + apply simplify_match_output in duo; subst. eauto.
 Defined.
 
-#[global] Program Instance VCCS_gLts : gLts proc VCCS_ExtAction := 
+(* #[global] Program Instance VCCS_gLts : gLts proc VCCS_ExtAction := 
   {| lts_step x ℓ y  := lts x ℓ y ;
      lts_state_eqdec := proc_dec ;
      lts_step_decidable p α q := lts_dec p α q ;
@@ -4456,16 +4456,25 @@ Defined.
      lts_refuses_decidable p α := proc_stable_dec p α 
     |}.
 Next Obligation.
-  intros p [[a|a]|]; intro hs;eapply gset_nempty_ex in hs as (r & l); eapply lts_set_spec0 in l; 
+  intros p [[a|a]|]; intro hs. eapply gset_nempty_ex in hs as (r & l). ; eapply lts_set_spec0 in l; 
   exists r; assumption.
 Qed.
 Next Obligation.  
   intros p [[a|a]|]; intros (q & mem); intro eq; eapply lts_set_spec1 in mem; set_solver.
-Qed.
+Qed. *)
 
 #[global] Program Instance VCCS_gLtsEq : gLtsEq proc VCCS_ExtAction := 
-  {| eq_rel x y  := cgr x y;
-     eq_spec p q α := Congruence_Respects_Transition p q α |}.
+  {| eq_rel x y  := cgr x y; |}.
+Next Obligation.
+  eapply (@MkgLts proc (ExtAct TypeOfActions) VCCS_ExtAction lts proc_dec
+  lts_dec proc_stable proc_stable_dec).
+  + intros p [[a|a]|]; intro hs; eapply gset_nempty_ex in hs as (r & l) ; eapply lts_set_spec0 in l; 
+    exists r; assumption.
+  + intros p [[a|a]|]; intros (q & mem); intro eq; eapply lts_set_spec1 in mem; set_solver.
+Defined.
+Next Obligation.
+  eapply Congruence_Respects_Transition.
+Defined.
 
 #[global] Program Instance VCCS_gLtsOBA : gLtsOba proc.
 Next Obligation.
@@ -5174,7 +5183,7 @@ Proof.
           eapply lts_refuses_spec2. exists p'1. eapply lts_choiceR. eauto.
 Qed.
 
-#[global] Program Instance AbsVCCS : AbsAction (ExtAct TypeOfActions) VCCS_ExtAction Φᴠᴄᴄꜱ 𝝳ᴠᴄᴄꜱ.
+#[global] Program Instance AbsVCCS : @AbsAction proc proc FinA PreAct (ExtAct TypeOfActions) VCCS_ExtAction Φᴠᴄᴄꜱ 𝝳ᴠᴄᴄꜱ _ VCCS_gLtsEq.
 Next Obligation.
   intros. destruct β; destruct β'; destruct a; destruct a0.
   - inversion H1; subst.
